nola/rust_lang/tactics.v
@@ -15,6 +15,7 @@ Inductive expr : Set :=
 | Var (x : string)
 | Lit (l : base_lit)
 | Rec (f : binder) (xl : list binder) (e : expr)
+| UnOp (op : un_op) (e : expr)
 | BinOp (op : bin_op) (e1 e2 : expr)
 | App (e : expr) (el : list expr)
 | Read (o : order) (e : expr)
@@ -33,6 +34,7 @@ Fixpoint to_expr (e : expr) : lang.expr :=
   | Var x => lang.Var x
   | Lit l => lang.Lit l
   | Rec f xl e => lang.Rec f xl (to_expr e)
+  | UnOp op e => lang.UnOp op (to_expr e)
   | BinOp op e1 e2 => lang.BinOp op (to_expr e1) (to_expr e2)
   | App e el => lang.App (to_expr e) (map to_expr el)
   | Read o e => lang.Read o (to_expr e)
@@ -50,6 +52,7 @@ Ltac of_expr e :=
   | lang.Var ?x => constr:(Var x)
   | lang.Lit ?l => constr:(Lit l)
   | lang.Rec ?f ?xl ?e => let e := of_expr e in constr:(Rec f xl e)
+  | lang.UnOp ?op ?e => let e := of_expr e in constr:(UnOp op e)
   | lang.BinOp ?op ?e1 ?e2 =>
     let e1 := of_expr e1 in let e2 := of_expr e2 in constr:(BinOp op e1 e2)
   | lang.App ?e ?el =>
@@ -87,7 +90,7 @@ Fixpoint is_closed (X : list string) (e : expr) : bool :=
   | BinOp _ e1 e2 | Write _ e1 e2 | Free e1 e2 =>
     is_closed X e1 && is_closed X e2
   | App e el | Case e el => is_closed X e && forallb (is_closed X) el
-  | Read _ e | Alloc e | Fork e => is_closed X e
+  | UnOp _ e | Read _ e | Alloc e | Fork e => is_closed X e
   | CAS e0 e1 e2 => is_closed X e0 && is_closed X e1 && is_closed X e2
   | Ndnat => true
   end.
@@ -132,6 +135,7 @@ Fixpoint subst (x : string) (es : expr) (e : expr)  : expr :=
   | Lit l => Lit l
   | Rec f xl e =>
     Rec f xl $ if bool_decide (BNamed x ≠ f ∧ BNamed x ∉ xl) then subst x es e else e
+  | UnOp op e => UnOp op (subst x es e)
   | BinOp op e1 e2 => BinOp op (subst x es e1) (subst x es e2)
   | App e el => App (subst x es e) (map (subst x es) el)
   | Read o e => Read o (subst x es e)
@@ -278,6 +282,7 @@ Ltac reshape_expr e tac :=
   with go K e :=
   match e with
   | _ => tac K e
+  | UnOp ?op ?e => go (UnOpCtx op :: K) e
   | BinOp ?op ?e1 ?e2 =>
      reshape_val e1 ltac:(fun v1 => go (BinOpRCtx op v1 :: K) e2)
   | BinOp ?op ?e1 ?e2 => go (BinOpLCtx op e2 :: K) e1
